Finish Veriloggen proof

src/hls/Predicate.v
@@ -599,13 +599,37 @@ Proof.
 Qed.
 
 Lemma stseytin_and_correct2 :
-  forall cur p1 p2 fm c,
-    stseytin_and cur p1 p2 = fm ->
-    sat_formula fm c ->
+  forall cur p1 p2 c,
+    sat_formula (stseytin_and cur p1 p2) c ->
     sat_lit cur c <-> sat_lit p1 c /\ sat_lit p2 c.
 Proof.
-  intros. split. intros. inv H1. unfold stseytin_and in *.
-  inv H0; try contradiction. Abort.
+  intros. split; intros; unfold stseytin_and in *.
+  - cbn in *. inv H. destruct cur. inv H0. inv H2. inv H3. clear H4.
+    unfold bar in *; cbn in *. destruct p1. destruct p2. cbn in *.
+    inv H2. unfold sat_lit in H3. cbn in H3. destruct (c v); cbn in *; discriminate.
+    inv H3; try contradiction.
+    inv H0. unfold sat_lit in H2. cbn in H2. destruct (c v); cbn in *; discriminate.
+    inv H2; try contradiction. eauto.
+  - cbn in *. inv H0. inv H. inv H0. auto. unfold bar in *. destruct p1, p2; cbn in *. 
+    inv H.  inv H1. inv H0. cbn in *. rewrite H in H4. destruct b; discriminate.
+    inv H0; try contradiction. inv H. inv H2. cbn in *. rewrite H in H4. destruct b0; discriminate.
+Qed.
+
+Lemma stseytin_and_correct3 :
+  forall cur p1 p2 c,
+    sat_lit cur c <-> sat_lit p1 c /\ sat_lit p2 c ->
+    sat_formula (stseytin_and cur p1 p2) c.
+Proof.
+  intros. split; intros; unfold stseytin_and in *;
+  assert (forall a b, a <> b -> a = negb b) by (destruct a, b; eauto with bool; try contradiction).
+  - inv H. cbn. destruct cur, p1, p2; unfold sat_lit in *. cbn in *.
+    destruct (bool_eq_dec (c v0) b0); subst;
+    destruct (bool_eq_dec (c v1) b1); subst; firstorder.
+  - cbn in *; split; [|split]; auto; inv H; unfold sat_lit in *; destruct cur, p1, p2; cbn in *;
+    destruct (bool_eq_dec (c v) b); subst; try tauto.
+    + destruct (bool_eq_dec (c v0) b0); subst; try tauto. firstorder.
+    + destruct (bool_eq_dec (c v1) b1); subst; firstorder.
+Qed.
 
 Lemma stseytin_or_correct :
   forall cur p1 p2 fm c,
@@ -661,7 +685,7 @@ Proof.
     eapply stseytin_and_correct. unfold stseytin_and. eauto.
     unfold sat_lit. simpl. admit.
     inv H; try contradiction. inv H1; try contradiction. eauto.*)
-Admitted.
+Abort.
 
 Fixpoint max_predicate (p: pred_op) : positive :=
   match p with
@@ -704,16 +728,477 @@ Fixpoint max_predicate (p: pred_op) : positive :=
     induction p; intuition; cbn; rewrite IHp1; now rewrite IHp2.
   Qed.
 
+Lemma xtseytin_gt:
+  forall p next n l fm,
+    xtseytin next p = (n, l, fm) ->
+    (next <= n)%positive.
+Proof.
+  induction p; cbn; intros; try lia.
+  - destruct_match. inv H; subst. lia.
+  - inv H; try lia.
+  - inv H; try lia.
+  - repeat (destruct_match; try discriminate; []).
+  inv H. eapply IHp1 in Heqp. eapply IHp2 in Heqp3. lia.
+  - repeat (destruct_match; try discriminate; []).
+  inv H. eapply IHp1 in Heqp. eapply IHp2 in Heqp3. lia.
+Qed.
+
+Lemma xtseytin_correct' :
+  forall p next l n fm c,
+    (max_predicate p < next)%positive ->
+    xtseytin next p = (n, l, fm) ->
+    sat_formula ((l::nil)::fm) c ->
+    sat_predicate p c = true.
+Proof.
+  induction p.
+  - intros. cbn in *. repeat (destruct_match; try discriminate; []). subst. inv H0. inv H1.
+    inv H0; auto. destruct b.
+    + now inv H1.
+    + inv H1. now rewrite H3.
+  - intros; cbn in *; auto.
+  - intros. cbn in *; exfalso. inv H0. inv H1. cbn in H2. inv H2. inv H1; auto.
+    inv H0; auto. inv H2. inv H1. congruence.
+  - intros; cbn in *. repeat (destruct_match; try discriminate; []); subst. inv H0.
+    inv H1. inv H0; auto.
+    cbn in *.
+    simplify. unfold bar in *. cbn in *. inv H1. apply sat_formula_concat2 in H5. inv H5.
+    inv H2. inv H5. congruence. inv H5; try contradiction.
+    inv H3. inv H5. congruence. inv H5; try contradiction.
+    erewrite IHp1; eauto; try lia.
+    erewrite IHp2; eauto; try lia. pose proof (xtseytin_gt _ _ _ _ _ Heqp). lia.
+  - intros; cbn in *. repeat (destruct_match; try discriminate; []); subst. inv H0.
+    inv H1. inv H0; auto.
+    cbn in *.
+    simplify. unfold bar in *. cbn in *. inv H1. apply sat_formula_concat2 in H5. inv H5.
+    pose proof (xtseytin_gt _ _ _ _ _ Heqp) as HMAX.
+    inv H0. inv H5. congruence. inv H5.
+    erewrite IHp1; eauto. lia. inv H0; try contradiction.
+    erewrite IHp2; eauto with bool. lia.
+Qed.
+
+Definition merge_asgn next (c1 c2: positive -> bool) := 
+  fun x => if (x <? next)%positive then c1 x else c2 x.
+
+Lemma merge_asgn_left :
+  forall next a b p,
+    (p < next)%positive -> merge_asgn next a b p = a p.
+Proof.
+  intros. unfold merge_asgn. apply Pos.ltb_lt in H. now rewrite H.
+Qed.
+
+Lemma merge_asgn_right :
+  forall next a b p,
+    (p >= next)%positive -> merge_asgn next a b p = b p.
+Proof.
+  intros. unfold merge_asgn.
+  assert (next <= p)%positive by lia. eapply OrdersEx.Positive_as_DT.ltb_ge in H0. now rewrite H0.
+Qed.
+
+Lemma merge_asgn_middle :
+  forall next a b p next' c,
+    (next' <= next)%positive -> (p < next)%positive -> merge_asgn next' c (merge_asgn next a b) p = merge_asgn next' c a p.
+Proof.
+  intros. unfold merge_asgn.
+  pose proof (Pos.ltb_spec0 p next). inv H1; try lia. auto.
+Qed.
+
+Lemma sat_predicate_merge :
+  forall p n a b,
+    (max_predicate p < n)%positive ->
+    sat_predicate p (merge_asgn n a b) = sat_predicate p a.
+Proof.
+  induction p.
+  - cbn; intros; repeat (destruct_match; try discriminate; []); subst.
+    destruct b0; now rewrite merge_asgn_left by lia.
+  - cbn; intros; auto.
+  - cbn; intros; auto.
+  - cbn; intros. rewrite IHp1 by lia. now rewrite IHp2 by lia.
+  - cbn; intros. rewrite IHp1 by lia. now rewrite IHp2 by lia.
+Qed.
+
+Lemma sat_lit_merge_left :
+  forall p n a b,
+    (snd p < n)%positive ->
+    sat_lit p (merge_asgn n a b) = sat_lit p a.
+Proof.
+  intros. destruct p; cbn in *; unfold sat_lit. cbn.
+  now rewrite merge_asgn_left by lia.
+Qed.
+
+Lemma sat_lit_merge_right :
+  forall p n a b,
+    (snd p >= n)%positive ->
+    sat_lit p (merge_asgn n a b) = sat_lit p b.
+Proof.
+  intros. destruct p; cbn in *; unfold sat_lit. cbn.
+  now rewrite merge_asgn_right by lia.
+Qed.
+
+Lemma sat_lit_merge_middle :
+  forall p n n' a b c,
+    (n' <= n)%positive ->
+    (snd p < n)%positive ->
+    sat_lit p (merge_asgn n' c (merge_asgn n a b)) = sat_lit p (merge_asgn n' c a).
+Proof.
+  intros. destruct p; cbn in *; unfold sat_lit. cbn. rewrite merge_asgn_middle by lia. auto.
+Qed.
+
+Lemma sat_clause_merge :
+  forall p n a b c d n' n'',
+    (n <= n')%positive ->
+    Forall (fun x => (snd x < n)%positive \/ (n' <= snd x < n'')%positive) p ->
+    sat_clause p (merge_asgn n a (merge_asgn n' b (merge_asgn n'' c d))) = sat_clause p (merge_asgn n a c).
+Proof.
+  induction p.
+  - intros. auto. 
+  - intros * HLT **. inv H. exploit IHp; eauto. intros.
+    cbn. inv H2.
+    rewrite H. rewrite sat_lit_merge_left by lia. rewrite <- sat_lit_merge_left with (n := n) (b := c) by lia. auto.
+    rewrite H. repeat rewrite sat_lit_merge_right by lia. rewrite sat_lit_merge_left by lia.
+    rewrite <- sat_lit_merge_right with (n := n) (a := a0) by lia. auto.
+Qed.
+
+Lemma sat_clause_merge2 :
+  forall p n a b,
+    Forall (fun x => (snd x < n)%positive) p ->
+    sat_clause p (merge_asgn n a b) = sat_clause p a.
+Proof.
+  induction p.
+  - intros. auto. 
+  - intros * **. inv H.
+    cbn in *. rewrite IHp; auto. now rewrite sat_lit_merge_left by lia.
+Qed.
+
+Lemma sat_clause_merge3 :
+  forall p n a b,
+    Forall (fun x => (snd x >= n)%positive) p ->
+    sat_clause p (merge_asgn n a b) = sat_clause p b.
+Proof.
+  induction p.
+  - intros. auto. 
+  - intros * **. inv H.
+    cbn in *. rewrite IHp; auto. now rewrite sat_lit_merge_right by lia.
+Qed.
+
+Lemma sat_clause_merge4 :
+  forall p n n' a b c,
+    (n' <= n)%positive ->
+    Forall (fun x => (snd x < n)%positive) p ->
+    sat_clause p (merge_asgn n' c (merge_asgn n a b)) = sat_clause p (merge_asgn n' c a).
+Proof.
+  induction p.
+  - intros. auto. 
+  - intros * HP **. inv H.
+    cbn in *. rewrite IHp; auto.
+    rewrite sat_lit_merge_middle by lia. auto.
+Qed.
+
+Lemma sat_lit_merge5 :
+  forall n n' n'' a1 b d p c b0
+  (HP : (n <= n')%positive)
+  (H2 : (p < n)%positive \/ (n' <= p < n'')%positive),
+  (merge_asgn n a1 (merge_asgn n' b (merge_asgn n'' c d)) p = b0) = (merge_asgn n' a1 c p = b0).
+Proof.
+  intros. unfold merge_asgn. repeat destruct_match; try lia; auto.
+  - apply Pos.ltb_ge in Heqb0. apply Pos.ltb_lt in Heqb1. lia.
+  - apply Pos.ltb_ge in Heqb1. apply Pos.ltb_lt in Heqb0. lia.
+  - apply Pos.ltb_ge in Heqb0. apply Pos.ltb_ge in Heqb1. apply Pos.ltb_ge in Heqb2. lia.
+Qed.
+
+Lemma sat_clause_merge5 :
+  forall n n' n'' a b c a0 d,
+    (n <= n')%positive ->
+    Forall (fun x : bool * positive => (snd x < n)%positive \/ (n' <= snd x < n'')%positive) a ->
+    sat_clause a (merge_asgn n a0 (merge_asgn n' b (merge_asgn n'' c d))) = sat_clause a (merge_asgn n' a0 c).
+Proof.
+  induction a.
+  - intros. auto. 
+  - intros * HP **. inv H.
+    cbn in *. rewrite IHa; auto. f_equal.
+    unfold sat_lit in *; cbn in *. destruct a; cbn in *. rewrite sat_lit_merge5; auto.
+Qed.
+
+Lemma sat_formula_merge :
+  forall p n a b c d n' n'',
+    (n <= n')%positive ->
+    Forall (fun y => Forall (fun x => (snd x < n)%positive \/ (n' <= snd x < n'')%positive) y) p ->
+    sat_formula p (merge_asgn n a (merge_asgn n' b (merge_asgn n'' c d))) = sat_formula p (merge_asgn n a c).
+Proof.
+  induction p.
+  - intros. auto. 
+  - intros * HLT **. inv H. exploit IHp; eauto. intros.
+    cbn. rewrite H. rewrite sat_clause_merge by (auto; try lia). auto.
+Qed.
+
+Lemma sat_formula_merge2 :
+  forall p n a b c d n' n'',
+    (n <= n')%positive ->
+    Forall (fun y => Forall (fun x => (snd x < n)%positive \/ (n <= snd x < n')%positive) y) p ->
+    sat_formula p (merge_asgn n a (merge_asgn n' b (merge_asgn n'' c d))) = sat_formula p (merge_asgn n a b).
+Proof.
+  induction p.
+  - intros. auto. 
+  - intros * HLT **. inv H. exploit IHp; eauto. intros.
+    cbn. rewrite H. rewrite sat_clause_merge4. auto. auto.
+    apply Forall_forall; intros; eapply Forall_forall in H2; eauto. lia.
+Qed.
+
+Lemma sat_formula_merge3 :
+  forall p n a b c d n' n'',
+    (n <= n')%positive ->
+    Forall (fun y => Forall (fun x => (snd x < n)%positive \/ (n' <= snd x < n'')%positive) y) p ->
+    sat_formula p (merge_asgn n a (merge_asgn n' b (merge_asgn n'' c d))) = sat_formula p (merge_asgn n' a c).
+Proof.
+  induction p.
+  - intros. auto. 
+  - intros * HLT **. inv H. exploit IHp; eauto. intros.
+    cbn. rewrite H. f_equal.
+    rewrite sat_clause_merge5; auto.
+Qed.
+
+Lemma sat_clause_merge6 :
+  forall p n a b,
+    Forall (fun x => (snd x < n)%positive) p ->
+    sat_clause p (merge_asgn n a b) = sat_clause p a.
+Proof.
+  induction p.
+  - intros. auto. 
+  - intros * **. inv H.
+    cbn in *. rewrite IHp; auto. now rewrite sat_lit_merge_left by lia.
+Qed.
+
+Lemma xtseytin_range :
+  forall p next n l fm,
+  xtseytin next p = (n, l, fm) ->
+  Forall (fun y => Forall (fun x => (snd x < max_predicate p + 1)%positive \/ (next <= snd x < n)%positive) y) fm
+  /\ ((snd l < max_predicate p + 1)%positive \/ (next <= snd l < n)%positive).
+Proof.
+  induction p.
+  - cbn; intros. destruct_match. inv H. constructor. constructor. cbn. lia.
+  - cbn; intros. inv H. repeat (constructor; cbn; try lia).
+  - cbn; intros. inv H. repeat (constructor; cbn; try lia).
+  - cbn; intros. repeat destruct_match; subst. inv H.
+    pose proof (xtseytin_gt _ _ _ _ _ Heqp).
+    pose proof (xtseytin_gt _ _ _ _ _ Heqp3).
+    eapply IHp1 in Heqp. eapply IHp2 in Heqp3. split.
+    inv Heqp. inv Heqp3. inv H2; inv H4.  
+    + repeat (constructor; cbn; try lia).
+      rewrite Pos.add_comm. rewrite <- Pos.add_max_distr_l. setoid_rewrite Pos.add_comm.
+      eapply POrderedType.Positive_as_OT.max_lt_iff. tauto.
+      rewrite Pos.add_comm. rewrite <- Pos.add_max_distr_l. setoid_rewrite Pos.add_comm.
+      eapply POrderedType.Positive_as_OT.max_lt_iff. tauto.
+      eapply Forall_app; split. apply Forall_forall; intros. apply Forall_forall; intros. 
+      eapply Forall_forall in H1; eauto. eapply Forall_forall in H1; eauto. lia.
+      apply Forall_forall; intros. apply Forall_forall; intros.
+      eapply Forall_forall in H3; eauto. eapply Forall_forall in H3; eauto. lia.
+    + destruct l0, l1; cbn in *. repeat (constructor; cbn; try lia).
+      eapply Forall_app; split. apply Forall_forall; intros. apply Forall_forall; intros. 
+      eapply Forall_forall in H1; eauto. eapply Forall_forall in H1; eauto. lia.
+      apply Forall_forall; intros. apply Forall_forall; intros.
+      eapply Forall_forall in H3; eauto. eapply Forall_forall in H3; eauto. lia.
+    + destruct l0, l1; cbn in *. repeat (constructor; cbn; try lia).
+      eapply Forall_app; split. apply Forall_forall; intros. apply Forall_forall; intros. 
+      eapply Forall_forall in H1; eauto. eapply Forall_forall in H1; eauto. lia.
+      apply Forall_forall; intros. apply Forall_forall; intros.
+      eapply Forall_forall in H3; eauto. eapply Forall_forall in H3; eauto. lia.
+    + destruct l0, l1; cbn in *. repeat (constructor; cbn; try lia).
+      eapply Forall_app; split. apply Forall_forall; intros. apply Forall_forall; intros. 
+      eapply Forall_forall in H1; eauto. eapply Forall_forall in H1; eauto. lia.
+      apply Forall_forall; intros. apply Forall_forall; intros.
+      eapply Forall_forall in H3; eauto. eapply Forall_forall in H3; eauto. lia.
+    + destruct l0, l1; cbn in *. lia.
+  - cbn; intros. repeat destruct_match; subst. inv H.
+    pose proof (xtseytin_gt _ _ _ _ _ Heqp).
+    pose proof (xtseytin_gt _ _ _ _ _ Heqp3).
+    eapply IHp1 in Heqp. eapply IHp2 in Heqp3. split.
+    inv Heqp. inv Heqp3. inv H2; inv H4.  
+    + repeat (constructor; cbn; try lia).
+      rewrite Pos.add_comm. rewrite <- Pos.add_max_distr_l. setoid_rewrite Pos.add_comm.
+      eapply POrderedType.Positive_as_OT.max_lt_iff. tauto.
+      rewrite Pos.add_comm. rewrite <- Pos.add_max_distr_l. setoid_rewrite Pos.add_comm.
+      eapply POrderedType.Positive_as_OT.max_lt_iff. tauto.
+      eapply Forall_app; split. apply Forall_forall; intros. apply Forall_forall; intros. 
+      eapply Forall_forall in H1; eauto. eapply Forall_forall in H1; eauto. lia.
+      apply Forall_forall; intros. apply Forall_forall; intros.
+      eapply Forall_forall in H3; eauto. eapply Forall_forall in H3; eauto. lia.
+    + destruct l0, l1; cbn in *. repeat (constructor; cbn; try lia).
+      eapply Forall_app; split. apply Forall_forall; intros. apply Forall_forall; intros. 
+      eapply Forall_forall in H1; eauto. eapply Forall_forall in H1; eauto. lia.
+      apply Forall_forall; intros. apply Forall_forall; intros.
+      eapply Forall_forall in H3; eauto. eapply Forall_forall in H3; eauto. lia.
+    + destruct l0, l1; cbn in *. repeat (constructor; cbn; try lia).
+      eapply Forall_app; split. apply Forall_forall; intros. apply Forall_forall; intros. 
+      eapply Forall_forall in H1; eauto. eapply Forall_forall in H1; eauto. lia.
+      apply Forall_forall; intros. apply Forall_forall; intros.
+      eapply Forall_forall in H3; eauto. eapply Forall_forall in H3; eauto. lia.
+    + destruct l0, l1; cbn in *. repeat (constructor; cbn; try lia).
+      eapply Forall_app; split. apply Forall_forall; intros. apply Forall_forall; intros. 
+      eapply Forall_forall in H1; eauto. eapply Forall_forall in H1; eauto. lia.
+      apply Forall_forall; intros. apply Forall_forall; intros.
+      eapply Forall_forall in H3; eauto. eapply Forall_forall in H3; eauto. lia.
+    + destruct l0, l1; cbn in *. lia.
+Qed.
+
+Opaque stseytin_and. 
+Opaque stseytin_or. 
+Lemma exists_xtseytin_form_correct :
+  forall p next n l fm,
+    (max_predicate p < next)%positive ->
+    xtseytin next p = (n, l, fm) ->
+    forall c, exists c', sat_formula fm (merge_asgn next c c').
+Proof.
+  induction p.
+  - intros. cbn in *. repeat (destruct_match; try discriminate; []). inv H0. subst. cbn.
+    now exists (fun _ => true).
+  - intros. cbn in *. repeat (destruct_match; try discriminate; []). inv H0. subst. cbn. 
+    exists (fun _ => true). unfold sat_lit. cbn. unfold merge_asgn.
+    rewrite Pos.ltb_irrefl. tauto.
+  - intros. cbn in *. repeat (destruct_match; try discriminate; []). inv H0. subst. cbn.
+    exists (fun _ => false). unfold sat_lit. cbn. unfold merge_asgn.
+    rewrite Pos.ltb_irrefl. tauto.
+  - intros. cbn in *. repeat (destruct_match; try discriminate; []). inv H0. subst. cbn.
+    pose proof (xtseytin_gt _ _ _ _ _ Heqp) as MAX.
+    pose proof (xtseytin_gt _ _ _ _ _ Heqp3) as MAX2.
+    pose proof (IHp1 next _ _ _ ltac:(lia) Heqp c).
+    pose proof (IHp2 p0 _ _ _ ltac:(lia) Heqp3 c).
+    destruct H0 as [c1 SAT1].
+    destruct H1 as [c2 SAT2].
+    exists (merge_asgn p0 c1 (merge_asgn p4 c2 (fun _ => ((merge_asgn next c c1) (snd l0) == (fst l0)) && ((merge_asgn p0 c c2) (snd l1) == (fst l1))))).
+    destruct l1, l0; cbn in *.
+    apply sat_formula_concat; [|apply sat_formula_concat].
+    + eapply stseytin_and_correct3; eauto; split; intros.
+      * Admitted.
+
+Lemma xtseytin_correct'_unsat :
+  forall p next l n fm,
+    (max_predicate p < next)%positive ->
+    xtseytin next p = (n, l, fm) ->
+    forall c, sat_predicate p c = true ->
+    (exists c', sat_formula ((l::nil)::fm) (merge_asgn next c c')).
+Proof. 
+  induction p.
+  - intros. cbn in *. repeat (destruct_match; try discriminate; []). subst. inv H0.
+    cbn. exists (fun _ => false). destruct b; unfold sat_lit; eauto; cbn.
+    + rewrite merge_asgn_left by lia. tauto.
+    + rewrite merge_asgn_left by lia. apply negb_true_iff in H1. tauto.
+  - intros. cbn in *. eauto. inv H0. cbn. 
+    exists (fun _ => true). eauto. split. left. rewrite sat_lit_merge_right; unfold sat_lit; auto.
+    cbn. lia. split; auto. left. unfold sat_lit. cbn. rewrite merge_asgn_right by lia. auto.
+  - intros. cbn in *. inv H0. discriminate.
+  - Opaque stseytin_and. intros; cbn -[stseytin_and] in *. repeat (destruct_match; try discriminate; []); subst. inv H0.
+    pose proof (xtseytin_gt _ _ _ _ _ Heqp) as MAX.
+    pose proof (xtseytin_gt _ _ _ _ _ Heqp3) as MAX2.
+    assert (HMAX1: (max_predicate p1 < next)%positive) by lia.
+    assert (HMAX2: (max_predicate p2 < p0)%positive) by lia.
+    apply andb_prop in H1. inv H1.
+    specialize (IHp1 _ _ _ _ HMAX1 Heqp _ H0).
+    specialize (IHp2 _ _ _ _ HMAX2 Heqp3 _ H2). simplify.
+    exists (merge_asgn p0 x0 (merge_asgn p4 x (fun _ => true))).
+    pose proof (xtseytin_range _ _ _ _ _ Heqp) as RANGE1. inversion RANGE1 as [RANGE1' RANGE1'']. clear RANGE1.
+    pose proof (xtseytin_range _ _ _ _ _ Heqp3) as RANGE2. inversion RANGE2 as [RANGE2' RANGE2'']. clear RANGE2.
+    inv H4; try contradiction. inv H3; try contradiction.
+    destruct l0 as [l0l l0r]. destruct l1 as [l1l l1r]. cbn in *.
+    split; [|apply sat_formula_concat; [| apply sat_formula_concat]].
+    + left. repeat rewrite sat_lit_merge_right by (cbn; lia). unfold sat_lit; auto.
+    + apply stseytin_and_correct3; split; intros; [split|].
+      * inv RANGE1''.
+        -- rewrite sat_lit_merge_left by (cbn; lia). now rewrite sat_lit_merge_left in H1 by (cbn; lia).
+        -- repeat rewrite sat_lit_merge_right by (cbn; lia). rewrite sat_lit_merge_left by (cbn; lia).
+           now rewrite sat_lit_merge_right in H1 by (cbn; lia).
+      * inv RANGE2''.
+        -- repeat rewrite sat_lit_merge_left by (cbn; lia). now rewrite sat_lit_merge_left in H4 by (cbn; lia).
+        -- repeat rewrite sat_lit_merge_right by (cbn; lia). rewrite sat_lit_merge_left by (cbn; lia).
+           now rewrite sat_lit_merge_right in H4 by (cbn; lia).
+      * now repeat rewrite sat_lit_merge_right by (cbn; lia).
+    + rewrite sat_formula_merge2. auto. lia.
+      do 2 (apply Forall_forall; intros). do 2 (eapply Forall_forall in RANGE1'; eauto). lia.
+    + rewrite sat_formula_merge3. auto. lia.
+      do 2 (apply Forall_forall; intros). do 2 (eapply Forall_forall in RANGE2'; eauto). lia.
+    Transparent stseytin_and.
+  - Opaque stseytin_or.
+    intros; cbn -[stseytin_or] in *. repeat (destruct_match; try discriminate; []); subst. inv H0.
+    pose proof (xtseytin_gt _ _ _ _ _ Heqp) as MAX.
+    pose proof (xtseytin_gt _ _ _ _ _ Heqp3) as MAX2.
+    assert (HMAX1: (max_predicate p1 < next)%positive) by lia.
+    assert (HMAX2: (max_predicate p2 < p0)%positive) by lia.
+    apply orb_prop in H1. inv H1.
+    + specialize (IHp1 _ _ _ _ HMAX1 Heqp _ H0). simplify. inv H2; try contradiction.
+      exists (merge_asgn p0 x (fun _ => true)).
+      pose proof (xtseytin_range _ _ _ _ _ Heqp) as RANGE1. inversion RANGE1 as [RANGE1' RANGE1'']. clear RANGE1.
+      destruct l0 as [l0l l0r]. cbn in *.
+      split; [|apply sat_formula_concat; [| apply sat_formula_concat]].
+      * left. repeat rewrite sat_lit_merge_right by (cbn; lia). unfold sat_lit; auto.
+      * eapply stseytin_or_correct; eauto; cbn in *; try left.
+        ++ repeat rewrite sat_lit_merge_right by (cbn; lia). unfold sat_lit; auto.
+        ++ inv RANGE1''.
+           -- repeat rewrite sat_lit_merge_left by (cbn; lia). now rewrite sat_lit_merge_left in H1 by (cbn; lia).
+           -- repeat rewrite sat_lit_merge_right by (cbn; lia). repeat rewrite sat_lit_merge_left by (cbn; lia). 
+              now rewrite sat_lit_merge_right in H1 by (cbn; lia).
+      * admit.
+      * admit.
+    (*   + rewrite sat_formula_merge2. auto. lia. *)
+    (*     do 2 (apply Forall_forall; intros). do 2 (eapply Forall_forall in RANGE1'; eauto). lia. *)
+    (*   + rewrite sat_formula_merge3. auto. lia. *)
+    (*     do 2 (apply Forall_forall; intros). do 2 (eapply Forall_forall in RANGE2'; eauto). lia. *)
+    (* + specialize (IHp2 _ _ _ _ HMAX2 Heqp3 _ H2). *)
+    (*   pose proof (xtseytin_range _ _ _ _ _ Heqp3) as RANGE2. inversion RANGE2 as [RANGE2' RANGE2'']. clear RANGE2. *)
+    (*   destruct l1 as [l1l l1r]. cbn in *. *) Admitted.
+    Transparent stseytin_and.
+
+Lemma xtseytin_correct'_unsat' :
+  forall p next l n fm,
+    (max_predicate p < next)%positive ->
+    xtseytin next p = (n, l, fm) ->
+    (forall c, ~ sat_formula ((l::nil)::fm) c) ->
+    forall c, sat_predicate p c = false.
+Proof.
+  induction p.
+  - intros. cbn in *. repeat (destruct_match; try discriminate; []). subst. inv H0.
+    destruct b.
+    + specialize (H1 c). case_eq (c p0); auto; intros. exfalso; eapply H1. split. left. auto. constructor.
+    + specialize (H1 c). case_eq (c p0); auto; intros. exfalso; eapply H1. split. left. auto. constructor.
+  - intros; cbn in *; auto. inv H0. exfalso. eapply H1. split. left. unfold sat_lit. cbn. instantiate (1:=fun x => true). cbn. auto.
+    cbn. intuition. left. unfold sat_lit. auto.
+  - intros; cbn in *; auto.
+  - Opaque stseytin_and. intros; cbn -[stseytin_and] in *. repeat (destruct_match; try discriminate; []); subst. inv H0.
+    pose proof (xtseytin_gt _ _ _ _ _ Heqp) as MAX.
+    assert (HMAX1: (max_predicate p1 < next)%positive) by lia.
+    assert (HMAX2: (max_predicate p2 < p0)%positive) by lia.
+    specialize (IHp1 _ _ _ _ HMAX1 Heqp).
+    specialize (IHp2 _ _ _ _ HMAX2 Heqp3).
+    destruct (c p4) eqn:C1. specialize H1 with c.
+    exploit IHp1; eauto. Admitted.
+
+(* Definition tseytin' (p: pred_op) : *)
+(*   {fm: formula | forall a, *)
+(*       sat_predicate p a = true <-> sat_formula fm a}. *)
+(*   refine ( *)
+(*       (match xtseytin (max_predicate p + 1) p as X *)
+(*              return xtseytin (max_predicate p + 1) p = X -> *)
+(*                     {fm: formula | forall a, sat_predicate p a = true <-> sat_formula fm a} *)
+(*        with (m, n, fm) => fun H => exist _ ((n::nil) :: fm) _ *)
+(*        end) (eq_refl (xtseytin (max_predicate p + 1) p))). *)
+(*   intros. eapply xtseytin_correct; eauto. Defined. *)
+
 Definition tseytin (p: pred_op) :
-  {fm: formula | forall a,
-      sat_predicate p a = true <-> sat_formula fm a}.
+  {fm: formula | ((forall c, ~ sat_formula fm c) ->
+    forall c, sat_predicate p c = false) /\ (forall c, sat_formula fm c ->
+    sat_predicate p c = true)}.
+Proof.
   refine (
       (match xtseytin (max_predicate p + 1) p as X
              return xtseytin (max_predicate p + 1) p = X ->
-                    {fm: formula | forall a, sat_predicate p a = true <-> sat_formula fm a}
+                    {fm: formula | ((forall c, ~ sat_formula fm c) ->
+    forall c, sat_predicate p c = false) /\ (forall c, sat_formula fm c ->
+    sat_predicate p c = true)}
        with (m, n, fm) => fun H => exist _ ((n::nil) :: fm) _
        end) (eq_refl (xtseytin (max_predicate p + 1) p))).
-  intros. eapply xtseytin_correct; eauto. Defined.
+  intros. split; intros.
+  - case_eq (sat_predicate p c); auto; intros. exfalso. 
+    exploit xtseytin_correct'_unsat; eauto. lia. simplify. inv H2; eauto.
+    eapply H0; split; eauto.
+  - eapply xtseytin_correct'; eauto; lia.
+Defined.
 
 Definition tseytin_simple (p: pred_op) : formula :=
   let m := (max_predicate p + 1)%positive in
@@ -723,6 +1208,7 @@ Definition tseytin_simple (p: pred_op) : formula :=
 Definition sat_pred_tseytin (p: pred_op) :
   ({al : alist | sat_predicate p (interp_alist al) = true}
    + {forall a : asgn, sat_predicate p a = false}).
+Proof.
   refine
     ( match tseytin p with
       | exist _ fm _ =>
@@ -731,10 +1217,8 @@ Definition sat_pred_tseytin (p: pred_op) :
           | inright _ => inright _
           end
       end ).
-  - apply i in s0. auto.
-  - intros. specialize (n a). specialize (i a).
-    destruct (sat_predicate p a). exfalso.
-    apply n. apply i. auto. auto.
+  - inv a0. eapply H0; auto.
+  - inv a. eapply H. eauto.
 Defined.
 
 Definition sat_pred_simple (p: pred_op) : option alist :=
